src/tls/TLS.Handshake.Transcript.fsti
@@ -69,6 +69,10 @@ module Psks = Parsers.OfferedPsks
 module CRF = Crypto.CRF
 
 //TODO: move to a separate module
+type sh13 = sh:HSM.sh{Negotiation.selected_version sh == Correct PV.TLS_1p3}
+type sh12 = sh:HSM.sh{Negotiation.selected_version sh == Correct PV.TLS_1p2}
+
+//TODO: move to a separate module
 let repr_hs12 (b:R.const_slice) =
   R.repr_p _ b HSM.handshake12_parser
 
@@ -201,14 +205,14 @@ type transcript_t =
 
   | Transcript12:
       ch:HSM.clientHello ->
-      sh:HSM.sh{Negotiation.selected_version sh == Correct PV.TLS_1p2} ->
+      sh:sh12 ->
       rest:bounded_list HSM.handshake12 max_transcript_size ->
       transcript_t
 
   | Transcript13:
       retried:option retry ->
       ch:HSM.clientHello ->
-      sh:HSM.sh{Negotiation.selected_version sh == Correct PV.TLS_1p3} ->
+      sh:sh13 ->
       rest:bounded_list HSM.handshake13 max_transcript_size ->
       transcript_t
 
@@ -629,7 +633,7 @@ val extract_hash
     (requires fun h0 ->
       invariant s tx h0 /\
       B.live h0 tag /\
-      B.(loc_disjoint (loc_buffer tag) (loc_region_only true Mem.tls_tables_region)) /\
+      B.(loc_disjoint (loc_buffer tag) (Mem.loc_tables_region ())) /\
       B.loc_disjoint (footprint s) (B.loc_buffer tag))
     (ensures fun h0 _ h1 ->
       let open B in
